

Appendix B

System of Equations

$$\sum F_y = 0 : R_{1,y} + F \sin(\theta) + R_{2,y} - P \sin(\theta) + R_{3,y} - \int_0^x \tilde{q}(x) d\tilde{x} = 0 \quad (\text{B.1})$$

$$\sum F_z = 0 : R_{1,z} + F \cos(\theta) + R_{2,z} - P \cos(\theta) + R_{3,z} = 0 \quad (\text{B.2})$$

$$M_z(l_a) = 0 : -R_{1,y}[l_a - x_1] + \int_0^{l_a} \int_0^x \tilde{q}(x) d\tilde{x} dx - F \sin(\theta)[l_a - x_{A_1}] - R_{2,y}[l_a - x_2] + P \sin(\theta)[l_a - x_{A_2}] - R_{3,y}[l_a - x_3] = 0 \quad (\text{B.3})$$

$$M_y(l_a) = 0 : -R_{1,z}[l_a - x_1] - F \cos(\theta)[l_a - x_{A_1}] - R_{2,z}[l_a - x_2] + P \cos(\theta)[l_a - x_{A_2}] - R_{3,z}[l_a - x_3] = 0 \quad (\text{B.4})$$

$$T_x(l_a) = 0 : - \int_0^{l_a} \tau(\tilde{x}) d\tilde{x} + R_{1,y}(z_h - \tilde{z}) + R_{2,y}(z_h - \tilde{z}) + R_{3,y}(z_h - \tilde{z}) - F \cos(\theta)(y_p) + F \sin(\theta)(0 - \tilde{z}) \\ + P \cos(\theta)(y_p) - P \sin(\theta)(0 - \tilde{z}) = 0$$

(B.5)

$$\frac{1}{EI_{zz}} \left(- \int_0^{x_1} \int_0^{x_b} \int_0^{x_a} \int_0^x \tilde{q}(x) d\tilde{x} dx_a dx_b dx_c \right) + C_1 x_1 + C_2 = d_1 \cos(\theta) \quad (\text{B.6})$$

$$\frac{1}{EI_{zz}} \left(\frac{R_{1,y}}{6} [x_2 - x_1]^3 - \int_0^{x_2} \int_0^{x_b} \int_0^{x_a} \int_0^x \tilde{q}(x) d\tilde{x} dx_a dx_b dx_c + \frac{F \sin(\theta)}{6} [x_2 - x_{A_1}]^3 \right) + C_1 x_2 + C_2 = 0 \quad (\text{B.7})$$

$$\begin{aligned} \frac{1}{EI_{zz}} & \left(\frac{R_{1,y}}{6} [x_3 - x_1]^3 - \int_0^{x_3} \int_0^{x_b} \int_0^{x_a} \int_0^x \tilde{q}(x) d\tilde{x} dx_a dx_b dx_c + \frac{F \sin(\theta)}{6} [x_3 - x_{A_1}]^3 \right. \\ & \left. + \frac{R_{2,y}}{6} [x_3 - x_2]^3 - \frac{P \sin(\theta)}{6} [x_3 - x_{A_2}]^3 \right) + C_1 x_3 + C_2 = d_3 \cos(\theta) \end{aligned} \quad (\text{B.8})$$

$$C_3 x_1 + C_4 = -d_1 \sin(\theta) \quad (\text{B.9})$$

$$\frac{1}{EI_{yy}} \left(\frac{R_{1,z}}{6} [x_2 - x_1]^3 + \frac{F \cos(\theta)}{6} [x_2 - x_{A_1}]^3 \right) + C_3 x_2 + C_4 = 0 \quad (\text{B.10})$$

$$\frac{1}{EI_{yy}} \left(\frac{R_{1,z}}{6} [x_3 - x_1]^3 + \frac{F \cos(\theta)}{6} [x_3 - x_{A_1}]^3 + \frac{R_{2,z}}{6} [x_3 - x_2]^3 - \frac{P \cos(\theta)}{6} [x_3 - x_{A_2}]^3 \right) + C_3 x_3 + C_4 = -d_3 \sin(\theta) \quad (\text{B.11})$$

$$\frac{1}{GJ} \left(- \int_0^x x_A \int_0^x \tau(\tilde{x}) d\tilde{x} dx + R_{1,y} (z_h - \tilde{z}) [x_A - x_1] \right) + C_5 = 0$$

(B.12)